Start fleshing out `pure_letrec_funProofTheory`

compiler/backend/proofs/pure_letrec_funProofScript.sml
@@ -3,12 +3,16 @@
 *)
 open HolKernel Parse boolLib bossLib BasicProvers;
 open arithmeticTheory listTheory alistTheory optionTheory pairTheory dep_rewrite
-     pred_setTheory relationTheory rich_listTheory finite_mapTheory;
+     pred_setTheory relationTheory rich_listTheory finite_mapTheory wordsTheory;
 open pure_expTheory pure_exp_lemmasTheory pure_exp_relTheory pure_evalTheory
      pure_congruenceTheory pure_miscTheory pure_eval_lemmasTheory
      pure_letrecTheory topological_sortTheory;
 
 val _ = new_theory "pure_letrec_funProof";
+
+val _ = temp_delsimps ["lift_disj_eq", "lift_imp_disj"]
+
+(******************** Definitions ********************)
 
 Definition Apps_def:
   Apps x [] = x ∧
@@ -53,48 +57,102 @@ Inductive body_rel:
      ~MEM f (freevars x) ⇒
      body_rel f args x (subst (make_subst args) x))
   ∧
-  (* this is the recursive call function: short form om LHS; long form on RHS *)
+  (* This is the recursive call function: short form on LHS; long form on RHS *)
   (∀xs ys.
      args_rel args xs ys ⇒
      body_rel f args (Apps (Var f) ys)
                      (Apps (Var f) xs))
   ∧
-  (* one must not bind the vars that are not to change *)
+  (* Lam - one must not bind the vars that are not to change *)
   (∀v x y.
      (∀n z. MEM (SOME (n,z)) args ⇒ v ≠ n) ∧
      body_rel f args x y ⇒
      body_rel f args (Lam v x) (Lam v y))
   ∧
+  (* Var - when we have a "constant" variable *)
+  (∀v w. MEM (SOME (v,w)) args ⇒
+    body_rel f args w (Var v))
+  ∧
+  (* Var - when we have a regular variable*)
+  (∀v.
+    (∀w. ¬ MEM (SOME (v,w)) args) ⇒
+    body_rel f args (Var v) (Var v))
+  ∧
   (* Prim *)
   (∀p xs ys.
      LIST_REL (body_rel f args) xs ys ⇒
      body_rel f args (Prim p xs) (Prim p ys))
-  (* TODO: fill in missing cases *)
+  ∧
+  (* Letrec - no shadowing, just as in Lam case *)
+  (∀xs x ys y.
+    (∀n z v. MEM (SOME (n,z)) args ∧ MEM v (MAP FST xs) ⇒ v ≠ n) ∧
+    MAP FST xs = MAP FST ys ∧
+    LIST_REL (body_rel f args) (MAP SND xs) (MAP SND ys) ∧
+    body_rel f args x y ⇒
+    body_rel f args (Letrec xs x) (Letrec ys y))
+  ∧
+  (* App (when not a recursive call) *)
+  (∀x1 x2 y1 y2.
+    (∀es. App x1 x2 ≠ Apps (Var f) es ∧ App y1 y2 ≠ Apps (Var f) es) ∧
+    body_rel f args x1 y1 ∧
+    body_rel f args x2 y2 ⇒
+    body_rel f args (App x1 x2) (App y1 y2))
 End
 
-Inductive letrec_rel:
+Inductive letrec_fun:
   (* this what the optimisation wants to achieve in reverse -- but it might
      not be provable directly ...
   (∀vs b b1 f args.
-    body_rel f args b b1 ∧
-    LENGTH args = LENGTH vs ∧ ALL_DISTINCT vs ∧
-    (∀n v. MEM (SOME (n,v)) args ⇒ v = Var n ∧ MEM n vs) ∧
-    closed (Letrec [(f,Lams vs b1)] x1) ∧
-    letrec_fun x x1 ⇒
-    letrec_fun (Let f (Lams vs (Letrec [(f,Lams vs1 b)] (Apps (Var f) (MAP Var vs1)))) x)
-               (Letrec [(f,Lams vs b1)] x1))
-  ∧
-    ... so how about this one instead: *)
-  (∀vs b b1 f args.
-    body_rel f args b b1 ∧
-    LENGTH args = LENGTH vs ∧ ALL_DISTINCT vs ∧
-    (∀n v. MEM (SOME (n,v)) args ⇒ MEM n vs) ∧
-    closed (Letrec [(f,Lams vs b1)] (Lams vs b1)) ⇒
+    body_rel f args a b ∧
+    ALL_DISTINCT vs ∧
+    LIST_REL (λa v. case a of NONE => T | SOME (n,w) => w = Var n ∧ n = v)) args vs
+    args_rel args (MAP Var vs) (MAP Var ws) ∧
+    closed (Letrec [(f,Lams vs b)] y) ∧
+    letrec_fun x y ⇒
     letrec_fun
-      (Letrec [(f,Lams vs1 (subst (make_subst args) b))]
-                 (Lams vs1 (subst (make_subst args) b)))
-      (Letrec [(f,Lams vs b1)] (Lams vs b1)))
+      (Let f (Lams vs (Letrec [(f,Lams ws a)] (Apps (Var f) (MAP Var ws)))) x)
+      (Letrec [(f,Lams vs b)] y))
+
+  i.e.:
+    Letrec map = λf xs. ... map f ys ... in
+    map g [a,b,c]
+  becomes:
+    Let map = (λf xs. (Letrec map = (λxs. ... map ys ...) in map xs)) in
+    map g [a,b,c]
+  because:
+    args = [SOME ("f", Var f); NONE] ⇒
+    args_rel args (MAP Var [f,ys]) (MAP Var [ys])
+    ∧
+    body_rel "map" args (... map f ys ...) (... map ys ...)
+      if no shadowing/other recursive calls etc.
+      by recursion + args_rel args (MAP Var [f,ys]) (MAP Var [ys])
+    ∧
+    letrec_fun (map g [a,b,c]) (map g [a,b,c]) ∧ LIST_REL ... args vs ∧ closed ...
+    trivially
+
+    ... so how about this one instead: *)
+  (∀vs ws a b f args.
+    body_rel f args a b ∧
+    ALL_DISTINCT vs ∧
+    args_rel args (MAP Var vs) (MAP Var ws) ∧
+    freevars (Lams vs b) ⊆ {f} ⇒
+    letrec_fun
+      (Letrec [(f,Lams ws (subst (make_subst args) a))]
+                 (Lams ws (subst (make_subst args) a)))
+      (Letrec [(f,Lams vs b)] (Lams vs b)))
   ∧
+  (∀vs ws a b f args xs ys.
+    body_rel f args a b ∧
+    args_rel args xs ys ∧
+    ALL_DISTINCT vs ∧
+    args_rel args (MAP Var vs) (MAP Var ws) ∧
+    freevars (Lams vs b) ⊆ {f} ⇒
+    letrec_fun
+      (Apps (Letrec [(f,Lams ws (subst (make_subst args) a))]
+                       (Lams ws (subst (make_subst args) a))) xs)
+      (Apps (Letrec [(f,Lams vs b)] (Lams vs b)) ys))
+  ∧
+
   (* cases below are just recursion *)
   (∀n.
     letrec_fun (Var n) (Var n))
@@ -108,24 +166,507 @@ Inductive letrec_rel:
     letrec_fun (App f x) (App g y))
   ∧
   (∀n xs ys.
-    LIST_REL (letrec_fun) xs ys ⇒
+    LIST_REL letrec_fun xs ys ⇒
     letrec_fun (Prim n xs) (Prim n ys))
   ∧
-  (∀xs y xs1 y1.
-    LIST_REL (letrec_fun) (MAP SND xs) (MAP SND xs1) ∧
-    MAP FST xs = MAP FST xs1 ∧ letrec_fun y y1 ⇒
-    letrec_fun (Letrec xs y) (Letrec xs1 y1))
+  (∀xs ys x y.
+    LIST_REL letrec_fun (MAP SND xs) (MAP SND ys) ∧
+    MAP FST xs = MAP FST ys ∧ letrec_fun x y ⇒
+    letrec_fun (Letrec xs x) (Letrec ys y))
 End
 
-Theorem Letrec_Lams:
-  body_rel f args b b1 ∧ LENGTH args = LENGTH vs ∧ ALL_DISTINCT vs ∧
-  (∀n v. MEM (SOME (n,v)) args ⇒ v = Var n ∧ MEM n vs) ∧
-  closed (Letrec [(f,Lams vs b1)] x1)
-  ⇒
-  Letrec [(f,Lams vs b1)] x ≅
-  Let f (Lams vs (Letrec [(f,Lams vs1 b)] (Apps (Var f) (MAP Var vs1)))) x
+
+(******************** Lemmas ********************)
+
+Theorem freevars_Lams[simp]:
+  ∀vs e. freevars (Lams vs e) = freevars e DIFF set vs
 Proof
-  cheat
+  Induct >> rw[Lams_def] >>
+  gvs[LIST_TO_SET_FILTER, INTER_DEF, EXTENSION] >>
+  metis_tac[]
 QED
+
+Theorem subst_Lams:
+  ∀l x f. subst f (Lams l x) = Lams l (subst (FDIFF f (set l)) x)
+Proof
+  Induct >> rw[Lams_def] >- simp[FDIFF_def, DRESTRICT_UNIV] >>
+  simp[subst_def, fdiff_fdomsub_INSERT]
+QED
+
+Theorem freevars_Apps[simp]:
+  ∀es e. freevars (Apps e es) = freevars e ∪ set (FLAT (MAP freevars es))
+Proof
+  Induct >> rw[Apps_def] >> simp[UNION_ASSOC]
+QED
+
+Theorem subst_Apps:
+  ∀l x f. subst f (Apps x l) = Apps (subst f x) (MAP (subst f) l)
+Proof
+  Induct >> rw[Apps_def, subst_def]
+QED
+
+Triviality Apps_SNOC_rewrite:
+  (∀x. Apps x [] = x) ∧
+  (∀ys x y. Apps x (SNOC y ys) = App (Apps x ys) y)
+Proof
+  conj_tac >- rw[Apps_def] >>
+  Induct >> rw[Apps_def]
+QED
+
+Theorem subst_make_subst_unchanged:
+    (∀n v. MEM (SOME (n,v)) args ⇒ v = Var n)
+  ⇒ subst (make_subst args) e = e
+Proof
+  rw[] >> irule subst_id >>
+  pop_assum mp_tac >> qid_spec_tac `args` >>
+  Induct >> rw[make_subst_def] >>
+  Cases_on `h` >> gvs[] >> Cases_on `x` >> gvs[FLOOKUP_UPDATE] >>
+  FULL_CASE_TAC >> gvs[]
+QED
+
+Theorem args_rel_LENGTH:
+  ∀l xs ys.
+    args_rel l xs ys
+  ⇒ LENGTH l = LENGTH xs ∧ LENGTH ys ≤ LENGTH l
+Proof
+  Induct_on `args_rel` >> rw[]
+QED
+
+Theorem args_rel_imp_LIST_REL:
+  ∀l xs ys.
+    args_rel l xs ys
+  ⇒ LIST_REL (λa x. case a of NONE => T | SOME (v,w) => Var v = x) l xs
+Proof
+  Induct_on `args_rel` >> rw[] >> gvs[MAP_EQ_CONS]
+QED
+
+Theorem args_rel_empty_args[simp]:
+  ∀xs ys. args_rel [] xs ys ⇔ xs = [] ∧ ys = []
+Proof
+  rw[Once args_rel_cases]
+QED
+
+Theorem body_rel_empty_args[simp]:
+  ∀f a b. body_rel f [] a b ⇒ a = b
+Proof
+  strip_tac >> Induct_on `body_rel` >> rw[make_subst_def] >>
+  gvs[LIST_REL_EL_EQN, EL_MAP] >> simp[LIST_EQ_REWRITE] >> rw[] >>
+  rename1 `n < _` >> first_x_assum drule >> strip_tac >>
+  Cases_on `EL n xs` >> Cases_on `EL n ys` >> gvs[] >>
+  last_x_assum mp_tac >> simp[Once LIST_EQ_REWRITE, EL_MAP] >>
+  disch_then drule >> simp[]
+QED
+
+Theorem letrec_fun_refl:
+  ∀x. letrec_fun x x
+Proof
+  recInduct freevars_ind >> rw[]
+  >- simp[Once letrec_fun_cases]
+  >- (
+    simp[Once letrec_fun_cases] >> disj2_tac >>
+    rw[LIST_REL_EL_EQN] >> first_x_assum irule >> simp[EL_MEM]
+    )
+  >- simp[Once letrec_fun_cases]
+  >- simp[Once letrec_fun_cases]
+  >- (
+    simp[Once letrec_fun_cases] >> ntac 2 disj2_tac >>
+    rw[LIST_REL_EL_EQN, EL_MAP] >> first_x_assum irule >>
+    qexists_tac `FST (EL n lcs)` >> simp[EL_MEM]
+    )
+QED
+
+(* TODO not sure if these are currently true *)
+Theorem letrec_fun_freevars:
+  ∀x y. letrec_fun x y ⇒ freevars x = freevars y
+Proof
+  cheat (* TODO *)
+QED
+
+Theorem letrec_fun_subst_single:
+  ∀x y a b s.
+    letrec_fun x y ∧ letrec_fun a b
+  ⇒ letrec_fun (subst s a x) (subst s b y)
+Proof
+  cheat (* TODO *)
+QED
+
+Theorem letrec_fun_subst:
+  ∀x y. letrec_fun x y ⇒
+    ∀f g. fmap_rel letrec_fun f g
+  ⇒ letrec_fun (subst f x) (subst g y)
+Proof
+  cheat (* TODO *)
+QED
+
+
+(******************** Theorems ********************)
+
+Theorem letrec_fun_correct:
+  letrec_fun a b ∧ closed a ∧ closed b ⇒ a ≃ b
+Proof
+  rw[] >> irule eval_to_sim_thm >> gvs[] >>
+  qexists_tac `letrec_fun` >> gvs[] >>
+  simp[eval_to_sim_def] >> rpt (pop_assum kall_tac) >>
+  simp[Once SWAP_FORALL_THM] >>
+  recInduct eval_wh_to_ind >> rw[]
+  >- (
+    rename1 `Lam v e` >>
+    qpat_x_assum `letrec_fun _ _` mp_tac >> simp[Once letrec_fun_cases] >> rw[]
+    >- (Cases_on `xs` using SNOC_CASES >> gvs[Apps_SNOC_rewrite]) >>
+    simp[eval_wh_to_def] >> rw[] >>
+    irule letrec_fun_subst_single >> simp[letrec_fun_refl]
+    )
+  >- (
+    rename1 `App a b` >>
+    qpat_x_assum `letrec_fun _ _` mp_tac >>
+    simp[Once letrec_fun_cases] >> reverse (rw[])
+    >- (
+      simp[eval_wh_to_def] >> IF_CASES_TAC >> gvs[] >- metis_tac[] >>
+      first_x_assum drule_all >> rw[] >>
+      Cases_on `dest_wh_Closure (eval_wh_to k a)` >> gvs[]
+      >- (qexists_tac `ck` >> Cases_on `eval_wh_to k a` >> gvs[]) >>
+      Cases_on `eval_wh_to k a` >> gvs[] >>
+      rename1 `eval_wh_to _ a = wh_Closure s ea` >>
+      rename1 `eval_wh_to _ g = wh_Closure _ eg` >>
+      IF_CASES_TAC >> gvs[]
+      >- (
+        qexists_tac `0` >> simp[] >> IF_CASES_TAC >> gvs[] >>
+        drule eval_wh_inc >> disch_then $ qspec_then `ck` $ assume_tac o GSYM >>
+        gvs[]
+        ) >>
+      gvs[bind_single_def] >>
+      last_x_assum $ qspec_then `subst s y eg` mp_tac >> impl_keep_tac
+      >- (
+        simp[closed_def] >> once_rewrite_tac[GSYM LIST_TO_SET_EQ_EMPTY] >>
+        DEP_REWRITE_TAC[freevars_subst] >> simp[SUBSET_DIFF_EMPTY, SUBSET_DEF] >>
+        imp_res_tac eval_wh_to_Closure_freevars_SUBSET >>
+        gvs[closed_def, NIL_iff_NOT_MEM] >>
+        irule letrec_fun_subst_single >> simp[]
+        ) >>
+      strip_tac >> gvs[] >>
+      Cases_on `eval_wh_to (k - 1) (subst s b ea) = wh_Diverge` >> gvs[]
+      >- (
+        qexists_tac `ck'` >> IF_CASES_TAC >> gvs[] >>
+        drule eval_wh_to_agree >>
+        disch_then $ qspec_then `ck + k` $ assume_tac o GSYM >> gvs[]
+        ) >>
+      qexists_tac `ck + ck'` >> gvs[] >>
+      qspecl_then [`ck + (ck' + k)`,`g`,`ck + k`] assume_tac eval_wh_inc >> gvs[] >>
+      qspecl_then [`ck + (ck' + k) - 1`,`subst s y eg`,`ck' + k - 1`]
+        assume_tac eval_wh_inc >>
+      gvs[] >>
+      Cases_on `eval_wh_to (k - 1) (subst s b ea)` >> gvs[]
+      ) >>
+    cheat (* TODO *)
+    )
+  >- (
+    rename1 `Letrec fns e` >>
+    qpat_x_assum `letrec_fun _ _` mp_tac >>
+    simp[Once letrec_fun_cases] >> reverse (rw[])
+    >- (
+      simp[eval_wh_to_def] >> IF_CASES_TAC >> gvs[]
+      >- (qexists_tac `0` >> simp[]) >>
+      last_x_assum irule >>
+      DEP_REWRITE_TAC[subst_funs_eq_subst] >> simp[] >>
+      DEP_REWRITE_TAC[IMP_closed_subst] >>
+      simp[FDOM_FUPDATE_LIST, MAP_MAP_o, combinTheory.o_DEF, LAMBDA_PROD] >>
+      simp[GSYM FST_THM] >> reverse (rpt conj_tac)
+      >- (
+        irule letrec_fun_subst >> simp[] >>
+        irule fmap_rel_FUPDATE_LIST_same >>
+        simp[MAP_MAP_o, combinTheory.o_DEF, LAMBDA_PROD] >> simp[GSYM FST_THM] >>
+        gvs[LIST_REL_EL_EQN, EL_MAP] >> rw[] >>
+        map_every qpat_abbrev_tac [`a = EL n fns`,`b = EL n ys`] >>
+        PairCases_on `a` >> PairCases_on `b` >> gvs[] >>
+        simp[Once letrec_fun_cases] >> disj2_tac >> disj2_tac >>
+        simp[LIST_REL_EL_EQN, EL_MAP] >> first_x_assum drule >> simp[]
+        ) >>
+      ho_match_mp_tac IN_FRANGE_FUPDATE_LIST_suff >> simp[] >>
+      simp[MAP_MAP_o, combinTheory.o_DEF, LAMBDA_PROD] >>
+      gvs[EVERY_MEM, MEM_MAP, PULL_EXISTS, FORALL_PROD] >> rw[] >> metis_tac[]
+      )
+    >- (
+      Cases_on `xs` using SNOC_CASES >> gvs[Apps_SNOC_rewrite] >>
+      imp_res_tac args_rel_LENGTH >> gvs[Lams_def, make_subst_def, Apps_def] >>
+      simp[eval_wh_to_def] >> IF_CASES_TAC >> gvs[]
+      >- (qexists_tac `0` >> simp[]) >>
+      last_x_assum irule >>
+      imp_res_tac body_rel_empty_args >> gvs[] >> csimp[letrec_fun_refl] >>
+      DEP_REWRITE_TAC[subst_funs_eq_subst, IMP_closed_subst] >> simp[] >>
+      simp[FDOM_FUPDATE_LIST] >>
+      ho_match_mp_tac IN_FRANGE_FUPDATE_LIST_suff >> simp[]
+      )
+    >- (
+      simp[eval_wh_to_def] >> IF_CASES_TAC >> gvs[]
+      >- (qexists_tac `0` >> simp[]) >>
+      first_x_assum irule >>
+      DEP_REWRITE_TAC[subst_funs_eq_subst, IMP_closed_subst] >>
+      simp[EVERY_MAP, FDOM_FUPDATE_LIST] >> rpt conj_tac
+      >- (ho_match_mp_tac IN_FRANGE_FUPDATE_LIST_suff >> simp[])
+      >- (ho_match_mp_tac IN_FRANGE_FUPDATE_LIST_suff >> simp[]) >>
+      irule letrec_fun_subst >> irule_at Any fmap_rel_FUPDATE_LIST_same >>
+      simp[] >> rw[]
+      >- (simp[Once letrec_fun_cases] >> disj1_tac >> metis_tac[]) >>
+      cheat (* TODO *)
+      )
+    ) >>
+  rename1 `Prim p xs` >>
+  qpat_x_assum `letrec_fun _ _` mp_tac >>
+  simp[Once letrec_fun_cases] >> rw[]
+  >- (
+    rename1 `Prim _ _ = _ _ zs` >>
+    Cases_on `zs` using SNOC_CASES >> gvs[Apps_SNOC_rewrite]
+    ) >>
+  Cases_on `p` >> gvs[eval_wh_to_def]
+  >- (
+    IF_CASES_TAC >> gvs[] >- (qexists_tac `0` >> gvs[]) >>
+    IF_CASES_TAC >> gvs[LIST_REL_EL_EQN] >>
+    `∃x1 x2 x3. xs = [x1;x2;x3]` by fs[LENGTH_EQ_NUM_compute] >>
+    `∃y1 y2 y3. ys = [y1;y2;y3]` by fs[LENGTH_EQ_NUM_compute] >>
+    gvs[wordsTheory.NUMERAL_LESS_THM, DISJ_IMP_THM, FORALL_AND_THM] >>
+    first_x_assum drule_all >> strip_tac >> gvs[] >>
+    reverse (Cases_on `eval_wh_to (k - 1) x1`) >> gvs[]
+    >- (qexists_tac `ck` >> gvs[])
+    >- (qexists_tac `ck` >> gvs[])
+    >- (qexists_tac `ck` >> gvs[])
+    >- (qexists_tac `ck` >> gvs[]) >>
+    reverse (IF_CASES_TAC) >> gvs[]
+    >- (
+      reverse (IF_CASES_TAC) >> gvs[]
+      >- (qexists_tac `ck` >> gvs[])
+      >- (
+        qexists_tac `ck` >> gvs[] >>
+        Cases_on `l` >> gvs[] >> Cases_on `ys'` >> gvs[]
+        ) >>
+      last_x_assum drule_all >> strip_tac >> gvs[] >>
+      reverse (Cases_on `eval_wh_to (k - 1) x3`) >> gvs[]
+      >- (
+        qexists_tac `ck'` >>
+        Cases_on `eval_wh_to (ck' + k - 1) y1 = wh_Diverge` >> gvs[] >>
+        drule eval_wh_to_agree >>
+        disch_then (qspec_then `ck + k - 1` assume_tac) >> gvs[]
+        ) >>
+      qspecl_then [`ck + ck' + k - 1`,`y1`,`ck + k - 1`] mp_tac eval_wh_inc >>
+      gvs[] >> strip_tac >>
+      qspecl_then [`ck + ck' + k - 1`,`y3`,`ck' + k - 1`] mp_tac eval_wh_inc >>
+      gvs[] >> strip_tac >>
+      qexists_tac `ck + ck'` >> gvs[]
+      )
+    >- (
+      qexists_tac `ck` >> gvs[] >>
+      Cases_on `l` >> gvs[] >> Cases_on `ys'` >> gvs[]
+      )
+    >- (
+      first_x_assum drule_all >> strip_tac >> gvs[] >>
+      reverse (Cases_on `eval_wh_to (k - 1) x2`) >> gvs[]
+      >- (
+        qexists_tac `ck'` >>
+        Cases_on `eval_wh_to (ck' + k - 1) y1 = wh_Diverge` >> gvs[] >>
+        drule eval_wh_to_agree >>
+        disch_then (qspec_then `ck + k - 1` assume_tac) >> gvs[]
+        ) >>
+      qspecl_then [`ck + ck' + k - 1`,`y1`,`ck + k - 1`] mp_tac eval_wh_inc >>
+      gvs[] >> strip_tac >>
+      qspecl_then [`ck + ck' + k - 1`,`y2`,`ck' + k - 1`] mp_tac eval_wh_inc >>
+      gvs[] >> strip_tac >>
+      qexists_tac `ck + ck'` >> gvs[]
+      )
+    )
+  >- (
+    IF_CASES_TAC >> gvs[] >> qexists_tac `0` >> simp[]
+    )
+  >- (
+    IF_CASES_TAC >> gvs[] >- (qexists_tac `0` >> simp[]) >>
+    IF_CASES_TAC >> gvs[] >> gvs[LIST_REL_EL_EQN] >>
+    `∃x. xs = [x]` by fs[LENGTH_EQ_NUM_compute] >>
+    `∃y. ys = [y]` by fs[LENGTH_EQ_NUM_compute] >>
+    gvs[wordsTheory.NUMERAL_LESS_THM] >>
+    first_x_assum drule_all >> rw[] >>
+    Cases_on `eval_wh_to (k - 1) x` >> gvs[] >>
+    qexists_tac `ck` >> gvs[] >>
+    IF_CASES_TAC >> gvs[] >>
+    IF_CASES_TAC >> gvs[]
+    )
+  >- (
+    IF_CASES_TAC >> gvs[] >- (qexists_tac `0` >> simp[]) >>
+    IF_CASES_TAC >> gvs[] >> gvs[LIST_REL_EL_EQN] >>
+    `∃x. xs = [x]` by fs[LENGTH_EQ_NUM_compute] >>
+    `∃y. ys = [y]` by fs[LENGTH_EQ_NUM_compute] >>
+    gvs[wordsTheory.NUMERAL_LESS_THM] >>
+    first_x_assum drule_all >> rw[] >>
+    reverse (Cases_on `eval_wh_to (k - 1) x`) >> gvs[]
+    >- (qexists_tac `ck` >> gvs[])
+    >- (qexists_tac `ck` >> gvs[])
+    >- (qexists_tac `ck` >> gvs[])
+    >- (qexists_tac `ck` >> gvs[]) >>
+    reverse IF_CASES_TAC >> gvs[]
+    >- (qexists_tac `ck` >> gvs[])
+    >- (qexists_tac `ck` >> gvs[]) >>
+    first_x_assum drule >> rw[] >>
+    last_x_assum drule >> impl_tac
+    >- (
+      gvs[closed_def, NIL_iff_NOT_MEM] >>
+      CCONTR_TAC >> gvs[] >>
+      imp_res_tac eval_wh_to_freevars_SUBSET >> gvs[MEM_MAP]
+      >- (
+        pop_assum kall_tac >> pop_assum mp_tac >> simp[PULL_EXISTS] >>
+        goal_assum drule >> simp[EL_MEM]
+        )
+      >- (
+        pop_assum mp_tac >> simp[PULL_EXISTS] >>
+        goal_assum drule >> simp[EL_MEM]
+        )
+      ) >>
+    rw[] >>
+    reverse (Cases_on `eval_wh_to (k - 1) (EL n l)`) >> gvs[]
+    >- (
+      qexists_tac `ck'` >>
+      Cases_on `eval_wh_to (ck' + k - 1) y = wh_Diverge` >> gvs[] >>
+      drule eval_wh_to_agree >>
+      disch_then (qspec_then `ck + k - 1` (assume_tac o GSYM)) >> gvs[]
+      ) >>
+    qspecl_then [`ck + ck' + k - 1`,`y`,`ck + k - 1`] mp_tac eval_wh_inc >>
+    gvs[] >> strip_tac >>
+    qspecl_then [`ck + ck' + k - 1`,`EL n ys'`,`ck' + k - 1`]
+      mp_tac eval_wh_inc >>
+    gvs[] >> strip_tac >>
+    qexists_tac `ck + ck'` >> gvs[]
+    )
+  >- (
+    IF_CASES_TAC >> gvs[] >- (qexists_tac `0` >> gvs[]) >>
+    CASE_TAC >> gvs[]
+    >- (
+      qsuff_tac `get_atoms (MAP (λa. eval_wh_to (k − 1) a) ys) = NONE`
+      >- (rw[] >> qexists_tac `0` >> simp[]) >>
+      gvs[get_atoms_NONE_eq] >> imp_res_tac LIST_REL_LENGTH >> gvs[] >>
+      csimp[EL_MAP] >> gvs[EL_MAP] >>
+      map_every (fn pat => qpat_x_assum pat mp_tac)
+        [`∀e1. MEM e1 _ ⇒ _`, `n < _`,`eval_wh_to _ _ = _`, `∀m. m < _ ⇒ _`,
+         `EVERY _ _`, `EVERY _ _`, `LENGTH _ = _`] >>
+      qid_spec_tac `n` >>
+      qpat_x_assum `LIST_REL _ _ _` mp_tac >>
+      map_every qid_spec_tac [`ys`,`xs`] >>
+      ho_match_mp_tac LIST_REL_ind >> rw[] >>
+      Cases_on `n` >> gvs[]
+      >- (
+        qexists_tac `0` >> gvs[] >>
+        first_x_assum (qspec_then `h1` mp_tac) >> simp[] >>
+        disch_then drule_all >> rw[] >>
+        CCONTR_TAC >> drule eval_wh_inc >>
+        disch_then (qspec_then `ck + k - 1` mp_tac) >> simp[]
+        ) >>
+      rename1 `n < _` >>
+      Cases_on `eval_wh_to (k - 1) h2 = wh_Diverge`
+      >- (qexists_tac `0` >> simp[]) >>
+      last_x_assum (qspec_then `n` mp_tac) >> simp[IMP_CONJ_THM] >>
+      impl_tac
+      >- (rw[] >> last_x_assum (qspec_then `SUC m` mp_tac) >> simp[]) >>
+      strip_tac >> rename1 `l < _` >>
+      qexists_tac `SUC l` >> simp[] >> rw[] >>
+      Cases_on `m` >> gvs[] >>
+      last_x_assum (qspec_then `0` assume_tac) >> gvs[] >>
+      first_x_assum (qspec_then `h1` mp_tac) >> simp[] >>
+      disch_then drule_all >> strip_tac >>
+      drule eval_wh_to_agree >>
+      disch_then (qspec_then `ck + k - 1` mp_tac) >> rw[] >>
+      metis_tac[]
+      ) >>
+    Cases_on `x` >> gvs[]
+    >- (
+      gvs[get_atoms_SOME_NONE_eq, EL_MAP] >>
+      qsuff_tac
+        `∃ck. get_atoms (MAP (λa. eval_wh_to (ck + k − 1) a) ys) = SOME NONE`
+      >- (rw[] >> qexists_tac `ck` >> simp[]) >>
+      simp[get_atoms_SOME_NONE_eq] >> csimp[EL_MAP] >>
+      imp_res_tac LIST_REL_LENGTH >> gvs[] >> goal_assum drule >>
+      map_every (fn pat => qpat_x_assum pat mp_tac)
+        [`∀e1. MEM e1 _ ⇒ _`, `n < _`,` ∀a. eval_wh_to _ _ ≠ _`,
+         `∀m. m ≤ _ ⇒ _`, `EVERY _ _`, `EVERY _ _`, `LENGTH _ = _`] >>
+      qid_spec_tac `n` >>
+      qpat_x_assum `LIST_REL _ _ _` mp_tac >>
+      map_every qid_spec_tac [`ys`,`xs`] >>
+      ho_match_mp_tac LIST_REL_ind >> rw[] >>
+      Cases_on `n` >> gvs[]
+      >- (
+        pop_assum (qspec_then `h1` mp_tac) >> simp[] >>
+        disch_then drule_all >> strip_tac >>
+        qexists_tac `ck` >>
+        Cases_on `eval_wh_to (k - 1) h1` >> gvs[]
+        ) >>
+      rename1 `SUC n` >>
+      last_x_assum (qspec_then `n` mp_tac) >> simp[] >> impl_tac
+      >- (rw[] >> last_x_assum (qspec_then `SUC m` mp_tac) >> simp[]) >>
+      strip_tac >>
+      first_x_assum (qspec_then `h1` mp_tac) >> simp[] >>
+      disch_then drule_all >> strip_tac >>
+      qexists_tac `ck + ck'` >> rw[]
+      >- (
+        qpat_x_assum `∀a. _ ≠ wh_Atom a` (qspec_then `a` mp_tac) >>
+        first_x_assum (qspec_then `n` mp_tac) >> simp[] >> strip_tac >>
+        drule eval_wh_inc >>
+        disch_then (qspec_then `ck + (ck' + k) - 1` assume_tac) >> gvs[]
+        ) >>
+      Cases_on `m` >> gvs[]
+      >- (
+        qspecl_then [`ck + (ck' + k) - 1`,`h2`,`ck' + k - 1`]
+          assume_tac eval_wh_inc >>
+        gvs[] >>
+        full_case_tac >> gvs[] >>
+        last_x_assum (qspec_then `0` assume_tac) >> gvs[]
+        )
+      >- (
+        rename1 `m ≤ _` >>
+        first_x_assum drule >> strip_tac >>
+        drule eval_wh_inc >>
+        disch_then (qspec_then `ck + (ck' + k) - 1` assume_tac) >> gvs[]
+        )
+      ) >>
+    rename1 `SOME (SOME as)` >>
+    qsuff_tac
+      `∃ck. get_atoms (MAP (λa. eval_wh_to (ck + k − 1) a) ys) = SOME (SOME as)`
+    >- (rw[] >> qexists_tac `ck` >> simp[] >> CASE_TAC >> gvs[]) >>
+    gvs[get_atoms_SOME_SOME_eq, EVERY2_MAP] >>
+    map_every (fn pat => qpat_x_assum pat mp_tac)
+      [`∀e1. MEM e1 _ ⇒ _`, `LIST_REL _ _ _`, `EVERY _ _`, `EVERY _ _`] >>
+    qid_spec_tac `as` >>
+    qpat_x_assum `LIST_REL _ _ _` mp_tac >>
+    map_every qid_spec_tac [`ys`,`xs`] >>
+    ho_match_mp_tac LIST_REL_strongind >> rw[] >>
+    rename1 `LIST_REL _ _ as` >>
+    qsuff_tac
+      `∃ck. LIST_REL (λa a'. eval_wh_to (ck + k − 1) a = wh_Atom a') ys as`
+    >- (
+      pop_assum (qspec_then `h1` mp_tac) >> simp[] >>
+      disch_then drule_all >> rw[] >>
+      qexists_tac `ck + ck'` >>
+      qspecl_then [`ck + ck' + k - 1`,`h2`,`ck + k - 1`]
+        assume_tac eval_wh_inc >>
+      gvs[LIST_REL_EL_EQN] >> rw[] >>
+      qspecl_then [`ck + ck' + k - 1`,`EL n ys`,`ck' + k - 1`]
+        assume_tac eval_wh_inc >>
+      gvs[]
+      ) >>
+    last_x_assum irule >> simp[]
+    )
+  >- (
+    IF_CASES_TAC >> gvs[] >- (qexists_tac `0` >> gvs[]) >>
+    IF_CASES_TAC >> gvs[] >> IF_CASES_TAC >> gvs[]
+    )
+QED
+
+Theorem Letrec_Lams:
+  body_rel g args a b ∧
+  ALL_DISTINCT vs ∧
+  args_rel args (MAP Var vs) (MAP Var ws) ∧
+  closed (Letrec [(g,Lams vs b)] e)
+  ⇒ Letrec [(g,Lams vs b)] e ≅
+    Let g (Lams vs (Letrec [(g,Lams ws a)] (Apps (Var g) (MAP Var ws)))) e
+Proof
+  rw[] >> once_rewrite_tac[exp_eq_open_bisimilarity_freevars] >>
+  irule open_bisimilarity_suff >> rw[] >>
+  cheat (* TODO *)
+QED
+
+(**********)
 
 val _ = export_theory();
